Verbatim/state.v
@@ -12,13 +12,20 @@ Module Type STATE (Import R : regex.T).
   Parameter State : Type.
   Parameter defState : State.
   
-  Parameter mk_transition : regex -> (Sigma -> State -> State).
+  Parameter transition : Sigma -> State -> State.
+  
+  Fixpoint transition_list (bs : list Sigma) (fsm : State) : State :=
+    match bs with
+    | [] => fsm
+    | c :: cs => transition_list cs (transition c fsm)
+    end.
+  
   Parameter accepts : String -> State -> bool.
   Parameter accepting : State -> bool.
 
   Parameter accepts_nil: forall(fsm : State), accepting fsm = accepts [] fsm.
-  Parameter accepts_transition : forall cand a fsm e,
-      accepts cand ((mk_transition e) a fsm) = accepts (a :: cand) fsm.
+  Parameter accepts_transition : forall cand a fsm,
+      accepts cand (transition a fsm) = accepts (a :: cand) fsm.
 
   Parameter init_state : regex -> State.
   Parameter init_state_inv : State -> regex.
@@ -26,9 +33,8 @@ Module Type STATE (Import R : regex.T).
   Parameter invert_init_correct : forall r s,
       exp_match s (init_state_inv (init_state r)) <-> exp_match s r.
 
-  Parameter accepts_dt : forall z a e,
-      accepts z (init_state (derivative a e))
-      = accepts z ((mk_transition e) a (init_state e)).
+  Parameter accepting_dt_list : forall bs e,
+      accepting (transition_list bs (init_state e)) = accepting (init_state (derivative_list bs e)).
   
   Parameter accepts_matches : forall(s : String) (e : regex),
     true = accepts s (init_state e) <-> exp_match s e.
